verify/HLv1.v
@@ -9,8 +9,9 @@ Import Inductive62.
 
 Definition T0:N := 0.
 Ltac solve_hlin_nonhalt_T T :=
-  apply (decide_hlin_nonhalt_spec _ (config_arithseq T0) T);
-  vm_cast_no_check (eq_refl true).
+  apply (decide_hlin_nonhalt_spec (config_arithseq T0) T);
+  [ apply Config_WF_simple; reflexivity
+  | vm_cast_no_check (eq_refl true)].
 
 Ltac solve_hlin_nonhalt :=
   match goal with
